theories/LevelTwoNF.v
@@ -1,16 +1,11 @@
 From Prototype Require Import Prelude Sig LevelTwo.
 
 (** This file defines normal forms of level two expressions [nf],
-    as well as a function [reduce] which computes normal forms. *)
+    as well as a function [normalize] which computes normal forms. *)
 
 Module Make (S : Sig).
 Module T := LevelTwo.Make (S).
 Import T.
-
-#[local] Notation "↑ k" := (T_sshift k) (at level 0).
-#[local] Notation "t .: s" := (T_scons t s) (at level 60, right associativity).
-#[local] Notation "s1 >> s2" := (T_scomp s1 s2) (at level 50, left associativity).
-#[local] Notation "t '[:' s ']'" := (T_subst t s) (at level 15, s at level 0, no associativity).
 
 (*********************************************************************************)
 (** *** Normal forms. *)
@@ -19,317 +14,484 @@ Import T.
 (** A term/substitution is in normal form if and only if:
     - metavariables always appear to the left of a substitution or composition.
     - no other term appears to the left of a substitution or composition. *)
-Inductive nf : forall {k s}, term k s -> Prop :=
-| nf_tvar {n} (i : fin n) : 
-    nf (T_var i)
-| nf_tctor {n} c (args : term _ (S1 n)) : 
-    nf args -> nf (T_ctor c args) 
-| nf_al_nil {n} : 
-    nf (@T_al_nil n)
-| nf_al_cons {n ty tys} (a : term (K_a ty) (S1 n)) (args : term (K_al tys) (S1 n)) :
-    nf a -> nf args -> nf (T_al_cons a args)
-| nf_abase {n} b x :
-    nf (@T_abase n b x) 
-| nf_aterm {n} (t : term K_t (S1 n)) :
-    nf t -> nf (T_aterm t)
-| nf_abind {n ty} (a : term (K_a ty) (S1 (S n))) :
-    nf a -> nf (T_abind a)
-| nf_sshift {n k} : 
-    nf (@T_sshift n k)
-| nf_scons {n m} (t : term K_t (S1 m)) (s : term K_s (S2 n m)) : 
+Inductive nf : forall {k s}, expr k s -> Prop :=
+| nf_tvar (i : nat) : 
+    nf (E_var i)
+| nf_tctor c (al : args _) : 
+    nf al -> nf (E_ctor c al) 
+| nf_al_nil : 
+    nf E_al_nil
+| nf_al_cons {ty tys} (a : arg ty) (al : args tys) :
+    nf a -> nf al -> nf (E_al_cons a al)
+| nf_abase b x :
+    nf (E_abase b x) 
+| nf_aterm (t : term) :
+    nf t -> nf (E_aterm t)
+| nf_abind {ty} (a : arg ty) :
+    nf a -> nf (E_abind a)
+| nf_sshift {k} : 
+    nf (↑k)
+| nf_scons (t : term) (s : subst) : 
     nf t -> nf s -> nf (t .: s)
-| nf_subst_t {n m k} (xt : mvar k (S1 n)) (s : term K_s (S2 n m)) : 
-    nf s -> nf (T_mvar xt [: s ])
-| nf_subst_s {n m o k} (xs : mvar K_s (S2 (k + S n) m)) (s : term K_s (S2 m o)) :
-    nf s -> nf (T_var fin_zero [: ↑k >> T_mvar xs ][: s])
-| nf_scomp {n m o k} (xs : mvar K_s (S2 (k + n) m)) (s : term K_s (S2 m o)) :
-    nf s -> nf (↑k >> T_mvar xs >> s).
+| nf_subst_t {k} (xt : mvar k S1) (s : subst) : 
+    nf s -> nf (E_mvar xt [: s ])
+| nf_subst_s i (xs : mvar K_s S2) (s : subst) :
+    nf s -> nf (E_var i [: E_mvar xs >> s])
+| nf_scomp k (xs : mvar K_s S2) (s : subst) :
+    nf s -> nf (↑k >> E_mvar xs >> s).
 Hint Constructors nf : core.
 
-(** Technical detail: we need a type of renaming expression. *)
-Inductive rexp : forall {n m}, term K_s (S2 n m) -> Prop :=
-| rexp_shift {n k} : 
-    rexp (@T_sshift n k)
-| rexp_cons {n m} (i : fin m) (r : term K_s (S2 n m)) :
-    rexp r -> rexp (T_var i .: r).
+(** Technical detail: we need to describe a class of renaming expressions,
+    which are a subset of explicit renamings which don't contain metavariables. *)
+Inductive rexp : subst -> Prop :=
+| rexp_shift k : rexp (↑k)
+| rexp_cons i r : rexp r -> rexp (E_var i .: r).
 Hint Constructors rexp : core.
 
+(** Renaming expressions are in fact a subclass of normal forms. *)
+Lemma rexp_impl_nf r : rexp r -> nf r.
+Proof. intros H. induction H ; auto. Qed.
+
 (*********************************************************************************)
-(** *** Inversion lemmas. *)
+(** *** Inversion tactic. *)
 (*********************************************************************************)
 
-Lemma inv_nf_tctor {n} c (args : term (K_al _) (S1 n)) : 
-  nf (T_ctor c args) -> nf args.
-Proof. intros H. inv H. repeat apply Eqdep.EqdepTheory.inj_pair2 in H2. now subst. Qed.
+(** Rocq's inversion tactic doesn't work well on hypotheses of the form [nf _].
+    We thus prove a number of inversion lemmas by hand, and provide a custom
+    tactic [inv_nf] which recursively inverts all [nf _] hypotheses. *)
 
-Lemma inv_nf_al_cons {ty tys n} (a : term (K_a ty) (S1 n)) (args : term (K_al tys) (S1 n)) :
-  nf (T_al_cons a args) -> nf a /\ nf args.
-Proof. intros H. inv H. repeat apply Eqdep.EqdepTheory.inj_pair2 in H3, H5. now subst. Qed.
-
-Lemma inv_nf_aterm {n} (t : term K_t (S1 n)) :
-  nf (T_aterm t) -> nf t.
+Lemma inv_nf_ctor c (al : args _) : 
+  nf (E_ctor c al) -> nf al.
 Proof. intros H. inv H. repeat apply Eqdep.EqdepTheory.inj_pair2 in H1. now subst. Qed.
 
-Lemma inv_nf_abind {n ty} (a : term (K_a ty) (S1 (S n))) :
-  nf (T_abind a) -> nf a.
-Proof. intros H. inv H. repeat apply Eqdep.EqdepTheory.inj_pair2 in H2. now subst. Qed.
+Lemma inv_nf_al_cons {ty tys} (a : arg ty) (al : args tys) :
+  nf (E_al_cons a al) -> nf a /\ nf al.
+Proof. intros H. inv H. repeat apply Eqdep.EqdepTheory.inj_pair2 in H2, H3. now subst. Qed.
 
-Lemma inv_nf_subst_t {n m k} (t : term k (S1 n)) (s : term K_s (S2 n m)) :
+Lemma inv_nf_aterm (t : term) :
+  nf (E_aterm t) -> nf t.
+Proof. intros H. inv H. assumption. Qed.
+
+Lemma inv_nf_abind {ty} (a : arg ty) :
+  nf (E_abind a) -> nf a.
+Proof. intros H. inv H. apply Eqdep.EqdepTheory.inj_pair2 in H1. now subst. Qed.
+
+(** This inversion lemma is a bit complex, because there are two cases
+    and the second case is only possible when [t] is _not_ a substitution.
+    We can usually use one of the simpler lemmas below. *)
+Lemma inv_nf_subst {k} (t : expr k S1) (s : subst) :
   nf (t[: s ]) -> 
-    (exists xt, t = T_mvar xt /\ nf s) \/ 
-    (match k as k0 return forall n, term k0 (S1 n) -> Prop with 
-     | K_t => fun n t =>
-       exists l (xs : mvar K_s (S2 (l + S n) n)), 
-         t = @T_var (S n) (@fin_zero n) [: @T_sshift (S n) l >> T_mvar xs ] /\ nf s
-     | _ => fun _ _ => False
-     end) n t.
+    (exists xt, t = E_mvar xt /\ nf s) \/ 
+    (match k as k0 return expr k0 S1 -> Prop with 
+     | K_t => fun t => exists l xs s', t = E_var l /\ s = E_mvar xs >> s' /\ nf s'
+     | _ => fun _ => False
+     end) t.
 Proof.
 intros H. inv H.
-- left. repeat apply Eqdep.EqdepTheory.inj_pair2 in H4, H5. subst. eauto.
-- right. repeat apply Eqdep.EqdepTheory.inj_pair2 in H6, H7. subst.
-  exists k0. exists xs0. split ; auto. 
-Admitted.
-
-Lemma inv_nf_scons {n m} (t : term K_t (S1 m)) (s : term K_s (S2 n m)) :
-  nf (t .: s) -> nf t /\ nf s.
-Proof. 
-intros H. inv H. 
-repeat apply Eqdep.EqdepTheory.inj_pair2 in H2.  
-repeat apply Eqdep.EqdepTheory.inj_pair2 in H3. now subst.
+- left. apply Eqdep.EqdepTheory.inj_pair2 in H0. subst. eauto.
+- right. apply Eqdep.EqdepTheory.inj_pair2 in H4. subst. eexists. eauto.
 Qed.
 
-Lemma inv_nf_scomp {n m o} (s1 : term K_s (S2 n m)) (s2 : term K_s (S2 m o)) :
-  nf (s1 >> s2) -> exists l xs, s1 = ↑l >> T_mvar xs /\ nf s2.
-Proof. intros H. inv H. repeat apply Eqdep.EqdepTheory.inj_pair2 in H4, H5. subst. eauto. Qed.
+Lemma inv_nf_scons (t : term) (s : subst) :
+  nf (t .: s) -> nf t /\ nf s.
+Proof. intros H. inv H. auto. Qed.
 
-Lemma inv_rexp_cons {n m} (i : fin m) (r : term K_s (S2 n m)) :
-  rexp (T_var i .: r) -> rexp r.
-Proof. intros H. inv H. repeat apply Eqdep.EqdepTheory.inj_pair2 in H4. now subst. Qed.
+Lemma inv_nf_scomp (s1 s2 : subst) :
+  nf (s1 >> s2) -> exists l xs, s1 = ↑l >> E_mvar xs /\ nf s2.
+Proof. intros H. inv H. eauto. Qed.
+
+Lemma inv_rexp_cons (i : nat) (r : subst) :
+  rexp (E_var i .: r) -> rexp r.
+Proof. intros H. inv H. assumption. Qed.
+
+Lemma inv_nf_subst_var i s : 
+  nf (E_var i [: s ]) -> 
+    exists (xs : mvar K_s S2) (s' : subst), s = E_mvar xs >> s' /\ nf s'.
+Proof. 
+intros H. apply inv_nf_subst in H.
+destruct H as [(xt & H3 & H4) | H2] ; [inv H3 |].
+destruct H2 as (l & xs & s' & H1 & H2 & H3).
+subst. eauto.
+Qed.
+
+Lemma inv_nf_subst_mvar {k} (xt : mvar k S1) s : 
+  nf (E_mvar xt [: s ]) -> nf s.
+Proof. 
+intros H. apply inv_nf_subst in H.
+destruct H as [(xt' & H3 & H4) | H2] ; [assumption|].
+dependent destruction k ; try easy.
+destruct H2 as (l & xs & s' & H1 & H2 & H3). inv H1.
+Qed.
+
+Lemma inv_nf_subst_ctor c al s : 
+  nf (E_ctor c al [: s ]) -> False.
+Proof. 
+intros H. apply inv_nf_subst in H.
+destruct H as [(xt & H3 & H4) | H2] ; [inv H3 |].
+destruct H2 as (l & xs & s' & H1 & H2 & H3). inv H1.
+Qed.
+
+Lemma inv_nf_subst_al_nil s : 
+  nf (E_al_nil [: s ]) -> False.
+Proof. 
+intros H. apply inv_nf_subst in H.
+destruct H as [(xt & H3 & H4) | H2] ; [inv H3 | auto].
+Qed.
+
+Lemma inv_nf_subst_al_cons {ty tys} (a : arg ty) (al : args tys) (s : subst) : 
+  nf (E_al_cons a al [: s ]) -> False.
+Proof. 
+intros H. apply inv_nf_subst in H.
+destruct H as [(xt & H3 & H4) | H2] ; [inv H3 | auto].
+Qed.
+
+Lemma inv_nf_subst_abase b x s : 
+  nf (E_abase b x [: s ]) -> False.
+Proof. 
+intros H. apply inv_nf_subst in H.
+destruct H as [(xt & H3 & H4) | H2] ; [inv H3 | auto].
+Qed.
+
+Lemma inv_nf_subst_aterm t s : 
+  nf (E_aterm t [: s ]) -> False.
+Proof. 
+intros H. apply inv_nf_subst in H.
+destruct H as [(xt & H3 & H4) | H2] ; [inv H3 | auto].
+Qed.
+
+Lemma inv_nf_subst_abind {ty} (a : arg ty) s : 
+  nf (E_abind a [: s ]) -> False.
+Proof. 
+intros H. apply inv_nf_subst in H.
+destruct H as [(xt & H3 & H4) | H2] ; [inv H3 | auto].
+Qed.
+
+Lemma inv_nf_subst_subst {k} (t : expr k S1) s1 s2 : 
+  nf (t [: s1 ] [: s2 ]) -> False.
+Proof. 
+intros H. apply inv_nf_subst in H.
+destruct H as [(xt & H3 & H4) | H2].
+- inv H3.
+- dependent destruction k ; auto. destruct H2 as (l & xs & s' & H1 & H2 & H3).
+  inv H1.
+Qed.
+
+(** Invert a single [nf _] hypothesis. We can extend this to handle more
+    cases as needed. *)
+Ltac inv_nf_once :=
+  match goal with 
+  | [ H : nf (E_ctor _ _) |- _ ] => apply inv_nf_ctor in H
+  | [ H : nf E_al_nil |- _ ] => clear H
+  | [ H : nf (E_al_cons _ _) |- _ ] => 
+    let H1 := fresh "H" in 
+    let H2 := fresh "H" in 
+    apply inv_nf_al_cons in H ;
+    destruct H as [H1 H2]
+  | [ H : nf (E_abase _ _) |- _ ] => clear H
+  | [ H : nf (E_aterm _) |- _ ] => apply inv_nf_aterm in H
+  | [ H : nf (E_abind _) |- _ ] => apply inv_nf_abind in H
+  | [ H : nf (↑_) |- _ ] => clear H
+  | [ H : nf (_ .: _) |- _ ] => apply inv_nf_scons in H
+  | [ H : nf (_ >> _) |- _ ] => 
+    apply inv_nf_scomp in H ;
+    let l := fresh "l" in 
+    let xs := fresh "xs" in 
+    let H1 := fresh "H" in 
+    let H2 := fresh "H" in 
+    destruct H as (l & xs & H1 & H2)
+  | [ H : nf (E_var _ [: _ ]) |- _ ] =>
+    apply inv_nf_subst_var in H ; 
+    let xs := fresh "xs" in 
+    let s := fresh "s" in 
+    let H1 := fresh "H" in 
+    let H2 := fresh "H" in 
+    destruct H as (xs & s & H1 & H2)
+  | [ H : nf (_ [: _ ]) |- _ ] =>
+    first [ now apply inv_nf_subst_ctor in H 
+          | now apply inv_nf_subst_al_nil in H 
+          | now apply inv_nf_subst_al_cons in H 
+          | now apply inv_nf_subst_abase in H 
+          | now apply inv_nf_subst_aterm in H 
+          | now apply inv_nf_subst_abind in H
+          | now apply inv_nf_subst_subst in H
+          | apply inv_nf_subst_mvar in H
+          | apply inv_nf_subst in H ]
+  end.
+
+(** Recursively invert all hypotheses of the form [nf _]. *)
+Ltac inv_nf := repeat inv_nf_once.
 
 (*********************************************************************************)
-(** *** Operations on normal forms. *)
+(** *** Normalization. *)
 (*********************************************************************************)
 
 (** Head of a normal form substitution. *)
-Equations head {n m} (s : term K_s (S2 (S n) m)) : term K_t (S1 m) :=
-head (↑ k) := T_var (fin_weaken k fin_zero) ;
+Equations head (s : subst) : term :=
+head (↑ k) := E_var k ;
 head (t .: _) := t ;
-head (↑k >> T_mvar xs >> s) := T_var fin_zero [: ↑k >> T_mvar xs ] [: s ] ;
-head s := T_var fin_zero [: s ].
+head (↑k >> E_mvar xs >> s) := E_var k [: E_mvar xs >> s ] ;
+head s := E_var 0 [: s ].
 
-Lemma head_sound {n m} (s : term K_s (S2 (S n) m)) :
-  head s =σ T_var fin_zero [: s ].
-Proof. funelim (head s) ; simp head in * ; auto. Qed.
+Lemma head_sound s : head s =σ E_var 0 [: s ].
+Proof. 
+funelim (head s) ; simp head in * ; auto.
+- rewrite aeq_sshift_var. now rewrite <-plus_n_O.
+- rewrite <-(aeq_subst_subst (E_var 0)), <-aeq_subst_subst.
+  apply e_subst_proper ; [|reflexivity].
+  rewrite <-aeq_subst_subst, aeq_sshift_var, <-plus_n_O.
+  reflexivity.    
+Qed.
 
-Lemma head_nf {n m} (s : term K_s (S2 (S n) m)) :
-  nf s -> nf (head s).
+Lemma head_rexp s : rexp s -> exists i, head s = E_var i.
+Proof. intros H. dependent elimination H ; simp head ; eauto. Qed.
+
+Lemma head_nf s : nf s -> nf (head s).
 Proof. intros H. dependent elimination H ; simp head ; auto. Qed.
 
-Definition cast_subst {n m m'} (e : m = m') (t : term K_s (S2 n m)) : term K_s (S2 n m') :=
-  match e with eq_refl => t end.
-
-Lemma cast_subst_K {n m} (e : m = m) (t : term K_s (S2 n m)) : 
-  cast_subst e t = t.
-Proof. pose proof (Eqdep_dec.UIP_refl_nat _ e) as ->. reflexivity. Qed.
-
-Lemma cast_subst_nf {n m m'} (e : m = m') (s : term K_s (S2 n m)) : 
-  nf s -> nf (cast_subst e s).
-Proof. subst. rewrite cast_subst_K. auto. Qed.
-
 (** Tail of a normal form substitution. *)
-Equations tail {n m} (s : term K_s (S2 (S n) m)) : term K_s (S2 n m) :=
-tail (↑k) := cast_subst _ (↑(S k)) ;
+Equations tail (s : subst) : subst :=
+tail (↑k) := ↑(S k) ;
 tail (_ .: s) := s ;
-tail (↑k >> T_mvar xs >> s) := cast_subst _ (↑(S k)) >> T_mvar xs >> s ;
+tail (↑k >> E_mvar xs >> s) := ↑(S k) >> E_mvar xs >> s ;
 tail s := ↑1 >> s.  
 
-Inductive seq :  -> Type := 
-| 
-
-Lemma tail_sound {n m} (s : term K_s (S2 (S n) m)) :
-  tail s =σ ↑1 >> s.
+Lemma tail_sound s : tail s =σ ↑1 >> s.
 Proof. 
 funelim (tail s) ; simp tail in * ; auto.
-- clear.
-  set (e := _ n k). clearbody e.
-  Set Printing Implicit.
-  set (t := _ n (S k)).
-  set (x := S k + n) in *.
-  assert (Ht : t =σ @T_sshift n (S k)) by reflexivity.
-  clearbody t.
-  clearbody x.
-
-- repeat rewrite aeq_assoc. now rewrite aeq_sshift_succ_l.
+- now rewrite aeq_sshift_succ_l.
+- repeat rewrite aeq_assoc. rewrite aeq_sshift_succ_l. reflexivity.
 Qed.
 
-Lemma tail_nf {n m} (s : term K_s (S2 (S n) m)) :
-  nf s -> nf (tail s).
+Lemma tail_rexp s : rexp s -> rexp (tail s).
+Proof. intros H. dependent elimination H ; simp tail ; auto. Qed.
+
+Lemma tail_nf s : nf s -> nf (tail s).
+Proof. intros H. dependent elimination H ; simp tail ; auto. Qed.
+
+(** Drop the first [k] elements of a substitution. *)
+Equations drop (k : nat) (s : subst) : subst :=
+drop 0 s := s ;
+drop (S k) s := tail (drop k s).
+
+Lemma drop_sound k s : drop k s =σ ↑k >> s.
 Proof. 
-intros H. dependent elimination H ; simp tail ; auto.
-- set (e := _ n k). clearbody e. 
-  set (x := k + S n) in *. clearbody x.
-  subst. cbn. apply (@nf_sshift n (S k)).
-- set (e := _ n k2). clearbody e.
-  set (x := k2 + S n) in *. clearbody x. 
-  subst. cbn. exact (nf_scomp xs0 s3 n21).
+funelim (drop k s) ; auto. rewrite tail_sound, H. 
+now rewrite aeq_assoc, aeq_sshift_succ_l.
 Qed.
+
+Lemma drop_rexp k s : rexp s -> rexp (drop k s).
+Proof. intros H. funelim (drop k s) ; auto. apply tail_rexp. auto. Qed.
+    
+Lemma drop_nf k s : nf s -> nf (drop k s).
+Proof. intros H. funelim (drop k s) ; auto. apply tail_nf. auto. Qed.
 
 (** Apply a normal form substitution to a variable. *)
-Equations subst_var_nf {n m} (i : fin n) (s : term K_s (S2 n m)) : term K_t (S1 m) :=
-subst_var_nf fin_zero s := head_nf s ;
-subst_var_nf (fin_succ i) s := subst_var_nf i (tail_nf s).
-
-Lemma subst_var_nf_sound {n m} (i : fin n) (s : term K_s (S2 n m)) :
-  subst_var_nf i s =σ T_var i [: s ].
+Definition vsubst (i : nat) (s : subst) : term :=
+  head (drop i s).
+  
+Lemma vsubst_sound i s : vsubst i s =σ E_var i [: s ].
 Proof. 
-funelim (subst_var_nf i s).
-- now rewrite head_nf_sound.
-- rewrite H. rewrite tail_nf_sound. rewrite <-aeq_subst_subst, aeq_sshift_var.
-  reflexivity.
+unfold vsubst. rewrite head_sound, drop_sound.
+rewrite <-aeq_subst_subst, aeq_sshift_var, <-plus_n_O. reflexivity.
 Qed.
 
-Lemma subst_var_nf_preserve {n m} (i : fin n) (s : term K_s (S2 n m)) :
-  nf s -> nf (subst_var_nf i s).
-Proof. 
-intros H. funelim (subst_var_nf i s) ; simp subst_var_nf.
-- now apply head_nf_preserve.
-- apply H. now apply tail_nf_preserve.
-Qed.
+Lemma vsubst_nf i s : nf s -> nf (vsubst i s).
+Proof. intros H. unfold vsubst. now apply head_nf, drop_nf. Qed.
 
-Axiom todo : forall {A}, A.
+Lemma vsubst_rexp i s : rexp s -> exists i', vsubst i s = E_var i'.
+Proof. intros H. unfold vsubst. apply head_rexp. now apply drop_rexp. Qed.
 
 (** Composition of renaming expressions. *)
-Equations comp_rexp {n m o} (r1 : term K_s (S2 n m)) (r2 : term K_s (S2 m o)) : term K_s (S2 n o) :=
-comp_rexp (@T_sshift n 0) (@T_scons ?(n) o (@T_var ?(o) i2) r2) := todo ;
-comp_rexp r1 r2 := r1 >> r2.
+Equations rcomp (r1 r2 : subst) : subst :=
+rcomp (↑k) r := drop k r  ;
+rcomp (E_var i .: r1) r2 := vsubst i r2 .: rcomp r1 r2  ;
+rcomp r1 r2 := r1 >> r2.
 
-(*
-↑k [>>] ↑1 := ↑(S k)
-(t .: s) [>>] ↑1 := t [ ↑1 ] .: s [>>] ↑1
-(n^ζ >> s) [>>] ↑1 := n^ζ >> (s [>>] ↑1)
+Lemma rcomp_sound r1 r2 : rcomp r1 r2 =σ r1 >> r2.
+Proof. funelim (rcomp r1 r2) ; simp drop ; auto.
+- now rewrite drop_sound.
+- now rewrite H, vsubst_sound, aeq_distrib.
+Qed.  
 
-i[↑1] := fin_succ i
-
-
-*)
-
-Inductive nf_ren : 
-
-(** Apply a normal form substitution to a normal form term. *)
-Equations subst_nf {k n m} (t : term k (S1 n)) (s : term K_s (S2 n m)) : term k (S1 m) by struct t :=
-subst_nf (T_var i) s := subst_var_nf i s ;
-subst_nf (T_ctor c args) s := T_ctor c (subst_nf args s) ;
-subst_nf T_al_nil _ := T_al_nil ;
-subst_nf (T_al_cons a args) s := T_al_cons (subst_nf a s) (subst_nf args s) ;
-subst_nf (T_abase b x) s := T_abase b x ;
-subst_nf (T_aterm t) s := T_aterm (subst_nf t s) ;
-subst_nf (T_abind a) s := T_abind (subst_nf a (T_var fin_zero .: s >> ↑1 (*scomp_nf s (↑1)*) )) ;
-subst_nf (T_subst t s1) s2 := T_subst t (scomp_nf s1 s2) ;
-subst_nf (T_mvar xt) s := T_subst (T_mvar xt) s
-(** Compose normal form substitutions. *)
-with scomp_nf {n m o} (s1 : term K_s (S2 n m)) (s2 : term K_s (S2 m o)) : term K_s (S2 n o) by struct s1 :=
-scomp_nf (↑k) s := (↑k) >> s ;
-scomp_nf (t1 .: s1) s2 := subst_nf t1 s2 .: scomp_nf s1 s2 ;
-scomp_nf (s1 >> s1') s2 := s1 >> (scomp_nf s1' s2) ;
-scomp_nf (T_mvar xs) s := (T_mvar xs) >> s.
-
-Lemma subst_scomp_nf_sound :
-  (forall k n m (t : term k (S1 n)) (s : term K_s (S2 n m)), subst_nf t s =σ t[: s ]) *
-  (forall n m o (s1 : term K_s (S2 n m)) (s2 : term K_s (S2 m o)), scomp_nf s1 s2 =σ s1 >> s2).
+Lemma rcomp_rexp r1 r2 : rexp r1 -> rexp r2 -> rexp (rcomp r1 r2).
 Proof. 
-apply subst_nf_elim with 
-  (P := fun _ _ _ t s res => res =σ t[: s ]) 
-  (P0 := fun _ _ _ s1 s2 res => res =σ s1 >> s2).
-- intros n m i s. now rewrite subst_var_nf_sound.
-- intros n m c args s ->. now rewrite aeq_subst_ctor.
-- intros n m s. now rewrite aeq_subst_al_nil.
-- intros ty tys n m a args s -> ->. now rewrite aeq_subst_al_cons.
-- intros b n m x s. now rewrite aeq_subst_abase.
-- intros n m t s ->. now rewrite aeq_subst_aterm.
-- intros ty n m a s ->. now rewrite aeq_subst_abind. 
-- intros k n m o t s1 s2 ->. now rewrite aeq_subst_subst.
-- reflexivity.
-- reflexivity.
-- intros n m o t1 s1 s2 -> ->. now rewrite aeq_distrib.
-- intros n m o p s1 s2 s3 ->. now rewrite aeq_assoc.
-- reflexivity.
+intros H1 H2. funelim (rcomp r1 r2) ; simp rcomp ; try (inv H1).
+- now apply drop_rexp.
+- destruct (vsubst_rexp i r2 H2) as [i' ->]. constructor.
+  apply inv_rexp_cons in H1. now apply H.
 Qed.
 
-Lemma subst_nf_sound {k n m} (t : term k (S1 n)) (s : term K_s (S2 n m)) :
-  subst_nf t s =σ t[: s ].
-Proof. apply subst_scomp_nf_sound. Qed.
-
-Lemma scomp_nf_sound {n m o} (s1 : term K_s (S2 n m)) (s2 : term K_s (S2 m o)) :
-  scomp_nf s1 s2 =σ s1 >> s2.
-Proof. apply subst_scomp_nf_sound. Qed.
+(** Lift a renaming expression through a binder. *)
+Definition up_rexp (r : subst) : subst :=
+  E_var 0 .: rcomp r (↑1).
   
+Lemma up_rexp_sound r : up_rexp r =σ up_subst r.
+Proof. unfold up_rexp. simp up_subst. now rewrite rcomp_sound. Qed.
 
-Lemma simpl_subst_nf {k n m} (t : term k (S1 n)) (s : term K_s (S2 n m)) :
-  nf t -> nf s -> nf (simpl_subst t s).
+Lemma up_rexp_rexp r : rexp r -> rexp (up_rexp r).
+Proof. intros H. unfold up_rexp. constructor. now apply rcomp_rexp. Qed. 
+
+(** Apply a renaming expression to a normal form term. *)
+Equations rsubst {k} (t : expr k S1) (r : subst) : expr k S1 :=
+rsubst (E_var i) r := vsubst i r ;
+rsubst (E_ctor c al) r := E_ctor c (rsubst al r) ;
+rsubst E_al_nil r := E_al_nil ;
+rsubst (E_al_cons a al) r := E_al_cons (rsubst a r) (rsubst al r) ;
+rsubst (E_abase b x) r := E_abase b x ;
+rsubst (E_aterm t) r := E_aterm (rsubst t r) ;
+rsubst (E_abind a) r := E_abind (rsubst a (up_rexp r)) ; 
+rsubst (E_mvar xt [: s ]) r := E_mvar xt [: sr_comp s r ] ;
+rsubst (E_var i [: E_mvar xs >> s]) r := E_var i [: E_mvar xs >> sr_comp s r ] ;
+rsubst t r := t [: r ]
+(** Compose a normal form substitution with a renaming expression. *)
+with sr_comp (s r : subst) : subst :=
+sr_comp (↑k) r := drop k r ;
+sr_comp (t .: s) r := rsubst t r .: sr_comp s r ;
+sr_comp (↑k >> E_mvar xs >> s) r := ↑k >> E_mvar xs >> sr_comp s r ;
+sr_comp s r := s >> r.
+
+Lemma rsubst_sr_comp_sound : 
+  (forall k t r, @rsubst k t r =σ t [: r ]) *
+  (forall s r, sr_comp s r =σ s >> r).
 Proof.
-apply simpl_subst_elim with (P0 := fun _ _ _ s1 s2 res => nf s1 -> nf s2 -> nf res) ;
-clear k n m t s.
-- intros n m i s H1 H2. now apply apply_subst_nf.
-- intros n m c args s H1 H2 H3. apply nf_tctor. apply H1 ; [|exact H3].
-  now apply inv_nf_tctor.
-- intros n m s H1 H2. apply nf_al_nil.
-- intros ty tys n m a args s H1 H2 H3 H4. apply inv_nf_al_cons in H3. apply nf_al_cons.
-  + now apply H1.
-  + now apply H2.
-- intros b n m x s H1 H2. apply nf_abase.
-- intros n m t s H1 H2 H3. apply inv_nf_aterm in H2. apply nf_aterm. now apply H1.
-- intros ty n m a s H1 H2 H3. apply inv_nf_abind in H2. apply nf_abind. apply H1.
-  + exact H2.
-  + admit.
-- intros k n m o t s1 s2 H1 H2 H3. 
-  inv H2.
-apply nf_subst_. 
+apply rsubst_elim with 
+  (P := fun _ t r res => res =σ t [: r ])
+  (P0 := fun s r res => res =σ s >> r).
+all: auto.
+- intros i r. now rewrite vsubst_sound.
+- intros c al r ->. now rewrite aeq_subst_ctor.
+- intros ty tys a al r -> ->. now rewrite aeq_subst_al_cons.
+- intros t r ->. now rewrite aeq_subst_aterm.
+- intros ty a r ->. rewrite up_rexp_sound. now rewrite aeq_subst_abind.
+- intros i xs s r ->. now rewrite aeq_subst_subst, aeq_assoc.
+- intros k xt s r ->. now rewrite aeq_subst_subst.
+- intros k r. now rewrite drop_sound.
+- intros t s r -> ->. now rewrite aeq_distrib.
+- intros k xs s r ->. now rewrite aeq_assoc.
+Qed.   
 
-Definition reduce {k s} (t : term k s) : term k s.
-dependent induction t.
-- exact (T_var f).
-- exact (T_ctor c IHt).
-- exact (T_al_nil).
-- exact (T_al_cons IHt1 IHt2).
-- exact (T_abase b d).
-- exact (T_aterm IHt).
-- exact (T_abind IHt).
-- exact (simpl_subst t1 t2).
-- exact (T_sshift k).
-- exact (T_scons IHt1 IHt2).
-- exact (T_scomp IHt1 IHt2).
-Defined.  
-
-Lemma up_subst_sid n : up_subst (@sid n) =σ sid.
+Lemma rsubst_sr_comp_nf : 
+  (forall k t r, nf t -> rexp r -> nf (@rsubst k t r)) *
+  (forall s r, nf s -> rexp r -> nf (sr_comp s r)).
 Proof. 
-cbv [up_subst sid]. simpl. setoid_rewrite <-(aeq_sshift_succ 0).
-setoid_rewrite aeq_sshift_scons. reflexivity.
-Qed.
+apply rsubst_elim with 
+  (P := fun _ t r res => nf t -> rexp r -> nf res)
+  (P0 := fun s r res => nf s -> rexp r -> nf res).
+all: try (intros ; inv_nf ; solve [ easy | intuition ]).
+- intros i r H1 H2. now apply vsubst_nf, rexp_impl_nf.
+- intros ty a r H1 H2 H3. inv_nf. constructor.
+  apply H1 ; auto. now apply up_rexp_rexp.
+- intros i xs s r H1 H2 H3. inv_nf. constructor. apply H1 ; auto. now inv H.
+- intros k r H1 H2. now apply drop_nf, rexp_impl_nf.
+Qed.      
 
-Lemma subst_sid k n (t : term k (S1 n)) : t[: sid] =σ t.
-Proof.
-dependent induction t generalizing n ; try (now auto).
-- unfold sid. rewrite (aeq_sshift_var f 0). reflexivity.
-- rewrite aeq_subst_ctor. rewrite IHt ; auto.
-- rewrite aeq_subst_al_cons. rewrite IHt1, IHt2 ; auto.
-- rewrite aeq_subst_aterm. rewrite IHt ; auto.
-- rewrite aeq_subst_abind. rewrite up_subst_sid. rewrite IHt ; auto.
-- setoid_rewrite aeq_subst_subst. rewrite aeq_sid_r. reflexivity.
+(** Lift a normal form substitution through a binder. *)
+Definition up_nf (s : subst) : subst := 
+  E_var 0 .: sr_comp s (↑1).
+
+Lemma up_nf_sound s : up_nf s =σ up_subst s.
+Proof. unfold up_nf. simp up_subst. now destruct rsubst_sr_comp_sound as [_ ->]. Qed.
+
+Lemma up_nf_nf s : nf s -> nf (up_nf s).
+Proof. 
+intros H. unfold up_nf. constructor ; auto. 
+destruct rsubst_sr_comp_nf as [_ H1]. auto. 
 Qed. 
 
-(** Main property: [reduce t] is axiomatically equal to [t]. *)
-Lemma reduce_sound {k s} (t : term k s) : reduce t =σ t.
-Proof.
-dependent induction t ; simpl ; try auto.
-- now rewrite simpl_subst_sound.
-- rewrite IHt1, IHt2. reflexivity.
-- rewrite IHt1, IHt2. reflexivity. 
+(** Apply a normal form substitution to a normal form term. *)
+Equations ssubst {k} (t : expr k S1) (r : subst) : expr k S1 :=
+ssubst (E_var i) s := vsubst i s ;
+ssubst (E_ctor c al) s := E_ctor c (ssubst al s) ;
+ssubst E_al_nil _ := E_al_nil ;
+ssubst (E_al_cons a al) s := E_al_cons (ssubst a s) (ssubst al s) ;
+ssubst (E_abase b x) _ := E_abase b x ;
+ssubst (E_aterm t) s := E_aterm (ssubst t s) ;
+ssubst (E_abind a) s := E_abind (ssubst a (up_nf s)) ; 
+ssubst (E_mvar xt [: s1 ]) s2 := E_mvar xt [: scomp s1 s2 ] ;
+ssubst (E_var i [: E_mvar xs >> s1]) s2 := E_var i [: E_mvar xs >> scomp s1 s2 ] ;
+ssubst t s := t [: s ]
+(** Compose two normal form substitutions. *)
+with scomp (s r : subst) : subst :=
+scomp (↑k) s := drop k s ;
+scomp (t .: s1) s2 := ssubst t s2 .: scomp s1 s2 ;
+scomp (↑k >> E_mvar xs >> s1) s2 := ↑k >> E_mvar xs >> scomp s1 s2 ;
+scomp s1 s2 := s1 >> s2.
+
+Lemma ssubst_scomp_sound :
+  (forall k (t : expr k S1) (s : subst), ssubst t s =σ t[: s ]) *
+  (forall (s1 s2 : subst), scomp s1 s2 =σ s1 >> s2).
+Proof. 
+apply ssubst_elim with 
+  (P := fun _ t s res => res =σ t[: s ]) 
+  (P0 := fun s1 s2 res => res =σ s1 >> s2).
+all: try reflexivity.
+- intros i s. now rewrite vsubst_sound.
+- intros c args s ->. now rewrite aeq_subst_ctor.
+- intros s. now rewrite aeq_subst_al_nil.
+- intros ty tys a args s -> ->. now rewrite aeq_subst_al_cons.
+- intros b x s. now rewrite aeq_subst_abase.
+- intros t s ->. now rewrite aeq_subst_aterm.
+- intros ty a s ->. now rewrite aeq_subst_abind, up_nf_sound. 
+- intros i xs s1 s2 ->. now rewrite aeq_subst_subst, aeq_assoc.
+- intros k xt s1 s2 ->. now rewrite aeq_subst_subst.
+- intros k s. now rewrite drop_sound.
+- intros t s1 s2 -> ->. now rewrite aeq_distrib.
+- intros k xs s1 s2 ->. now rewrite aeq_assoc.
 Qed.
 
-(*(** This lemma is a simple consequence of the soundness of [simpl]. 
-    We could also prove it directly by induction, e.g. if we need it to prove 
-    the soundness of [simpl]. *)
-#[global] Instance simpl_proper k s : Proper (axiom_eq ==> axiom_eq) (@simpl k s).
-Proof. intros ???. rewrite simpl_sound, simpl_sound. assumption. Qed.*)
+Lemma ssubst_scomp_nf :
+  (forall k (t : expr k S1) (s : subst), nf t -> nf s -> nf (ssubst t s)) *
+  (forall (s1 s2 : subst), nf s1 -> nf s2 -> nf (scomp s1 s2)).
+Proof. 
+apply ssubst_elim with 
+  (P := fun _ t s res => nf t -> nf s -> nf res) 
+  (P0 := fun s1 s2 res => nf s1 -> nf s2 -> nf res).
+all: try (intros ; inv_nf ; solve [ easy | intuition ]).
+- intros i s H1 H2. now apply vsubst_nf.
+- intros ty a s H1 H2 H3. constructor. inv_nf. apply H1 ; auto. now apply up_nf_nf.
+- intros i xs s1 s2 H1 H2 H3. constructor. inv_nf. apply H1 ; auto. now inv H.
+- intros k s H1 H2. now apply drop_nf.
+Qed.  
+
+(** Normalize a metavariable. *)
+Equations normalize_mvar {k s} (x : mvar k s) : expr k s :=
+@normalize_mvar K_s S2 xs := ↑0 >> E_mvar xs >> sid ;
+@normalize_mvar _ S1 xt := E_mvar xt [: sid ] ;
+@normalize_mvar _ _ x := E_mvar x. 
+
+Lemma normalize_mvar_sound {k s} (x : mvar k s) : 
+  normalize_mvar x =σ E_mvar x.
+Proof. funelim (normalize_mvar x) ; auto. now rewrite aeq_sid_l, aeq_sid_r. Qed.
+
+(** Reduce an expression to normal form. *)
+Equations normalize {k s} (e : expr k s) : expr k s :=
+normalize (E_var i) := E_var i ;
+normalize (E_ctor c al) := E_ctor c (normalize al) ;
+normalize E_al_nil := E_al_nil ;
+normalize (E_al_cons a al) := E_al_cons (normalize a) (normalize al) ;
+normalize (E_abase b x) := E_abase b x ;
+normalize (E_aterm t) := E_aterm (normalize t) ;
+normalize (E_abind a) := E_abind (normalize a) ;
+normalize (t [: s ]) := ssubst (normalize t) (normalize s) ;
+normalize (↑k) := ↑k ;
+normalize (t .: s) := normalize t .: normalize s ;
+normalize (s1 >> s2) := scomp (normalize s1) (normalize s2) ;
+normalize (E_mvar x) := normalize_mvar x.
+
+Lemma normalize_sound {k s} (e : expr k s) : normalize e =σ e.
+Proof.
+funelim (normalize e) ; try (now auto).
+- destruct ssubst_scomp_sound as [-> _]. now rewrite H, H0.
+- destruct ssubst_scomp_sound as [_ ->]. now rewrite H, H0.
+- now rewrite normalize_mvar_sound.
+Qed.
+
+Lemma normalize_nf {k s} (e : expr k s) : nf (normalize e).
+Proof.
+funelim (normalize e) ; try (now auto).
+- destruct ssubst_scomp_nf as [H1 _] ; apply H1 ; auto.
+- destruct ssubst_scomp_nf as [_ H1] ; apply H1 ; auto.
+- admit.
+Admitted.
 
 End Make.
